# baseURI: http://icdd.vm.rub.de/ontology/icdd2ams
# imports: http://asbing.de/condition/def/
# imports: http://www.roadotl.eu/def/
# imports: https://w3id.org/bot#
# prefix: icdd2ams

@prefix icdd2ams: <http://icdd.vm.rub.de/ontology/icdd2ams#> .
@prefix asbing: <http://asbing.de/condition/def/> .
@prefix bot: <https://w3id.org/bot#> .
@prefix eurotl: <http://www.roadotl.eu/def/> .
@prefix owl: <http://www.w3.org/2002/07/owl#> .
@prefix prov: <http://www.w3.org/ns/prov#> .
@prefix rdf: <http://www.w3.org/1999/02/22-rdf-syntax-ns#> .
@prefix rdfs: <http://www.w3.org/2000/01/rdf-schema#> .
@prefix xsd: <http://www.w3.org/2001/XMLSchema#> .
@prefix dcterms: <http://purl.org/dc/terms/> .
@prefix vann: <http://purl.org/vocab/vann/> .

icdd2ams:
  rdf:type owl:Ontology ;
  owl:imports asbing: ;
  owl:imports eurotl: ;
  owl:imports bot: ;
    vann:preferredNamespacePrefix "icdd2ams";
    dcterms:title "Asset Condition Integration from ICDD to AMS (icdd2ams)"^^xsd:string;
    dcterms:description "Ontology for integrating BOT located asset conditions using eurotl and asbing ontologies into sql based asset management systems"^^xsd:string ;
    dcterms:created "2021-03-24"^^xsd:date ;
    dcterms:creator "Philipp Hagedorn";
    dcterms:creator "Liu Liu";
    dcterms:license <https://creativecommons.org/licenses/by/4.0/>;
.

icdd2ams:hadActivity
  rdf:type owl:ObjectProperty ;
  rdfs:domain bot:Building ;
  rdfs:label "icdd2ams:hadActivity" ;
  rdfs:comment "The activity relation representing the inspection of a BOT building, using a eurotl InspectionActivity individual";
  rdfs:range eurotl:InspectionActivity ;
  rdfs:subPropertyOf prov:hadActivity ;
.

icdd2ams:hasCondition
  rdf:type owl:ObjectProperty ;
  rdfs:domain bot:Element ;
  rdfs:label "icdd2ams:hasCondition" ;
  rdfs:comment "The condition of an element regarding an inspection activity" ;
  rdfs:range eurotl:Condition ;
  rdfs:subPropertyOf eurotl:hasCondition ;
.